General tidy up, including replacing the odd and ad-hoc definition of DEL by a more conventional one (and thereby eliminating the need for REG and REGF). README file has been updated.
Some, but not all, of the "x" value simulation problems have now gone
away.

examples/dev/compile.sml
@@ -1471,7 +1471,7 @@ val MAKE_NETLIST =
 (* Compile a device implementation into a clocked circuit represented in HOL *)
 (*****************************************************************************)
 val at_thms =
- [UNDISCH REG_IMP,UNDISCH REGF_IMP,
+ [UNDISCH DEL_IMP,UNDISCH DELT_IMP,UNDISCH DELF_IMP,
   EQ_at,COMB_at,CONSTANT_at,TRUE_at,FALSE_at,
   NOT_at,AND_at,OR_at,MUX_at,
   EQ_at,ADD_at,SUB_at,LESS_at];
@@ -1483,7 +1483,7 @@ val MAKE_CIRCUIT =
  (I ## Ho_Rewrite.REWRITE_RULE[at_CONCAT])                                 o
  at_SPEC_ALL ``clk:num->bool``                                             o
  GEN_ALL                                                                   o
- Ho_Rewrite.REWRITE_RULE[GSYM LEFT_FORALL_IMP_THM,REG_CONCAT]              o
+ Ho_Rewrite.REWRITE_RULE[GSYM LEFT_FORALL_IMP_THM,DEL_CONCAT]              o
  CONV_RULE(RATOR_CONV(RAND_CONV EXISTS_OUT_CONV))                          o
  Ho_Rewrite.REWRITE_RULE 
   [COMB_NOT,COMB_AND,COMB_OR,COMB_ADD,COMB_SUB,COMB_LESS,COMB_EQ]          o
@@ -1491,8 +1491,8 @@ val MAKE_CIRCUIT =
   (RATOR_CONV(RAND_CONV(REDEPTH_CONV(COMB_SYNTH_CONV))))                   o
  SIMP_RULE std_ss [UNCURRY]                                                o
  Ho_Rewrite.REWRITE_RULE
-  [BUS_CONCAT_ELIM,DFF_IMP_def,POSEDGE_IMP_def,LATCH_def,
-   DEL_IMP_def,GSYM DEL_IMP_THM]                                           o
+  [BUS_CONCAT_ELIM,DFF_IMP_def,POSEDGE_IMP_def,LATCH_def
+   (*DEL_IMP_def,GSYM DEL_IMP_THM*)]                                           o
  DEV_IMP (DEPTH_IMP DFF_IMP_INTRO)                                         o
  Ho_Rewrite.REWRITE_RULE
    [FUN_EXISTS_PROD,LAMBDA_PROD,COMB_ID,COMB_CONSTANT_1,COMB_CONSTANT_2,
@@ -1507,7 +1507,7 @@ val MAKE_CIRCUIT =
  REWRITE_RULE 
   [POSEDGE_IMP,CALL,SELECT,FINISH,ATM,SEQ,PAR,ITE,REC,
    ETA_THM,PRECEDE_def,FOLLOW_def,PRECEDE_ID,FOLLOW_ID,
-   GSYM DEL_IMP_THM,DEL_IMP_def,
+   (*GSYM DEL_IMP_THM,DEL_IMP_def,*)
    Ite_def,Par_def,Seq_def,o_THM];
 
 
